@prefix dc: <http://purl.org/dc/elements/1.1/> .
@prefix ec: <http://w3id.org/hefquin/engineconf#> .
@prefix rdf: <http://www.w3.org/1999/02/22-rdf-syntax-ns#> .
@prefix rdfs: <http://www.w3.org/2000/01/rdf-schema#> .
@prefix xsd: <http://www.w3.org/2001/XMLSchema#> .
@prefix xsd1: <http://www.w3.org/2000/10/XMLSchema#> .

ec:ConstructorArgument a rdfs:Class ;
    rdfs:label "Constructor Argument"@en ;
    rdfs:comment "This class is a superclass of any kind of argument to be passed to the constructor of a corresponding Java class. Concrete types of arguments are captured by the subclasses of this class."@en .

ec:CostModel a rdfs:Class ;
    rdfs:label "Cost Model"@en ;
    rdfs:subClassOf ec:InstantiableJavaClass .

ec:DesignatedArgumentValue a rdfs:Class ;
    rdfs:label "Designated Argument Value"@en ;
    rdfs:comment "The instances of this class that are defined in this vocabulary can be referred to as values by a 'ValueBasedConstructorArgument'."@en .

ec:ExecutionEngine a rdfs:Class ;
    rdfs:label "Execution Engine"@en ;
    rdfs:subClassOf ec:InstantiableJavaClass .

ec:FederationAccessManager a rdfs:Class ;
    rdfs:label "Federation Access Manager"@en ;
    rdfs:subClassOf ec:InstantiableJavaClass .

ec:HeFQUINEngineConfiguration a rdfs:Class ;
    rdfs:label "HeFQUIN Engine Configuration"@en ;
    rdfs:comment "Class of configurations of the HeFQUIN engine. Instances of this class must have exactly one 'fedAccessMgr' property and one 'queryProcessor' property."@en .

ec:InstantiableJavaClass a rdfs:Class ;
    rdfs:label "Instantiable Java Class"@en ;
    rdfs:comment "Every instance of this class represents a Java class that can be instantiated based on the given RDF description. Instances of this class must have exactly one 'javaClassName' property. Additionally, they may have a 'constructorArguments' property."@en .

ec:InstantiationBasedConstructorArgument a rdfs:Class ;
    rdfs:label "Instantiation-Based Constructor Argument"@en ;
    rdfs:comment "Every instance of this class represents a Java object that is obtained by instantiating a Java class and that is meant to be passed to a constructor in order to instantiate another Java class. In addition to the 'javaClassName' property and the (optional) 'constructorArguments' property, every instance of this class must have exactly one 'argumentTypeName' property. The value of this property is either the same as the value of the 'javaClassName' property or it is the name of a superclass or an interface of the class mentioned by the 'javaClassName' property."@en ;
    rdfs:subClassOf ec:ConstructorArgument,
        ec:InstantiableJavaClass .

ec:ListBasedConstructorArgument a rdfs:Class ;
    rdfs:label "List-Based Constructor Argument"@en ;
    rdfs:comment "Every instance of this class represents a 'java.util.List' that is populated and then passed as an argument to the constructor of a corresponding Java class. Instances of this class must have exactly one 'elementsTypeName' property and exactly one 'elements' property. Each element of the 'rdf:List' that the latter property refers to is expected to be of type 'InstantiableJavaClass' and the values of their respective 'javaClassName' properties are expected to be either the same as the value of the 'elementsTypeName' property (of this 'ListBasedConstructorArgument') or the name of a sub-class of the class mentioned by the 'elementsTypeName' property."@en ;
    rdfs:subClassOf ec:ConstructorArgument .

ec:LogicalOptimizer a rdfs:Class ;
    rdfs:label "Logical Optimizer"@en ;
    rdfs:subClassOf ec:InstantiableJavaClass .

ec:PhysicalOptimizer a rdfs:Class ;
    rdfs:label "Physical Optimizer"@en ;
    rdfs:subClassOf ec:InstantiableJavaClass .

ec:PlanCompiler a rdfs:Class ;
    rdfs:label "Plan Compiler"@en ;
    rdfs:subClassOf ec:InstantiableJavaClass .

ec:QueryPlanner a rdfs:Class ;
    rdfs:label "Query Planner"@en ;
    rdfs:comment "Instances of this class must have exactly one 'sourcePlanner' property, one 'logicalOptimizer' property, one 'physicalOptimizer' property."@en .

ec:QueryProcessor a rdfs:Class ;
    rdfs:label "Query Processor"@en ;
    rdfs:comment "Instances of this class must have exactly one 'queryPlanner' property, one 'planCompiler' property, one 'executionEngine' property. Additionally, they may have a 'costModel' property."@en .

ec:SourcePlanner a rdfs:Class ;
    rdfs:label "Source Planner"@en ;
    rdfs:subClassOf ec:InstantiableJavaClass .

ec:ValueBasedConstructorArgument a rdfs:Class ;
    rdfs:label "Value-Based Constructor Argument"@en ;
    rdfs:comment "Every instance of this class refers to a concrete value to be passed as an argument to the constructor of a corresponding Java class. In particular, to refer to this value, instances of this class must have exactly one 'rdf:value' property. The value may be either a literal or any 'DesignatedArgumentValue' defined in this vocabulary."@en ;
    rdfs:subClassOf ec:ConstructorArgument .

ec:DefaultCostModel a ec:CostModel ;
    ec:constructorArguments ( [ ec:argumentTypeName "se.liu.ida.hefquin.engine.queryproc.impl.poptimizer.CardinalityEstimation" ;
                ec:constructorArguments ( [ rdf:value <http://w3id.org/hefquin/engineconf#value:QueryProcContext> ] ) ;
                ec:javaClassName "se.liu.ida.hefquin.engine.queryproc.impl.poptimizer.cardinality.CardinalityEstimationImpl" ] ) ;
    ec:javaClassName "se.liu.ida.hefquin.engine.queryproc.impl.poptimizer.costmodel.CostModelImpl" .

ec:DefaultExecutionEngine a ec:ExecutionEngine ;
    ec:constructorArguments () ;
    ec:javaClassName "se.liu.ida.hefquin.engine.queryproc.impl.execution.ExecutionEngineImpl" .

ec:DefaultFederationAccessManager a ec:FederationAccessManager ;
    ec:constructorArguments ( [ ec:argumentTypeName "se.liu.ida.hefquin.engine.federation.access.FederationAccessManager" ;
                ec:constructorArguments ( <http://w3id.org/hefquin/engineconf#value:ExecServiceForFedAccess> ) ;
                ec:javaClassName "se.liu.ida.hefquin.engine.federation.access.impl.AsyncFederationAccessManagerImpl" ] 100 ) ;
    ec:javaClassName "se.liu.ida.hefquin.engine.federation.access.impl.FederationAccessManagerWithCache" .

ec:DefaultLogicalOptimizer a ec:LogicalOptimizer ;
    ec:constructorArguments ( [ rdf:value <http://w3id.org/hefquin/engineconf#value:QueryProcContext> ] [ ec:elements ( [ ec:javaClassName "se.liu.ida.hefquin.engine.queryproc.impl.loptimizer.heuristics.MergeRequests" ] [ ec:javaClassName "se.liu.ida.hefquin.engine.queryproc.impl.loptimizer.heuristics.FilterPushDown" ] [ ec:javaClassName "se.liu.ida.hefquin.engine.queryproc.impl.loptimizer.heuristics.MergeRequests" ] [ ec:constructorArguments ( [ ec:argumentTypeName "se.liu.ida.hefquin.engine.queryproc.impl.loptimizer.heuristics.formula.FormulaForComputingSelectivity" ;
                                        ec:javaClassName "se.liu.ida.hefquin.engine.queryproc.impl.loptimizer.heuristics.formula.JoinAwareWeightedUnboundVariableCount" ] ) ;
                            ec:javaClassName "se.liu.ida.hefquin.engine.queryproc.impl.loptimizer.heuristics.GreedyBasedReordering" ] [ ec:javaClassName "se.liu.ida.hefquin.engine.queryproc.impl.loptimizer.ApplyVocabularyMappings" ] [ ec:constructorArguments ( <http://w3id.org/hefquin/engineconf#value:QueryProcContext> ) ;
                            ec:javaClassName "se.liu.ida.hefquin.engine.queryproc.impl.loptimizer.heuristics.CardinalityBasedJoinOrderingWithRequests" ] [ ec:javaClassName "se.liu.ida.hefquin.engine.queryproc.impl.loptimizer.heuristics.RemoveUnnecessaryL2gAndG2l" ] [ ec:javaClassName "se.liu.ida.hefquin.engine.queryproc.impl.loptimizer.heuristics.PullUpLtgOverUnion" ] [ ec:javaClassName "se.liu.ida.hefquin.engine.queryproc.impl.loptimizer.heuristics.PullUpLtgOverJoin" ] [ ec:javaClassName "se.liu.ida.hefquin.engine.queryproc.impl.loptimizer.heuristics.PushJoinUnderUnionWithRequests" ] [ ec:javaClassName "se.liu.ida.hefquin.engine.queryproc.impl.loptimizer.heuristics.PullUpLtgOverUnion" ] [ ec:javaClassName "se.liu.ida.hefquin.engine.queryproc.impl.loptimizer.heuristics.RemovePairsOfG2lAndL2g" ] ) ;
                ec:elementsTypeName "se.liu.ida.hefquin.engine.queryproc.impl.loptimizer.HeuristicForLogicalOptimization" ] ) ;
    ec:javaClassName "se.liu.ida.hefquin.engine.queryproc.impl.loptimizer.HeuristicsBasedLogicalOptimizerImpl" .

ec:DefaultPhysicalOptimizer a ec:PhysicalOptimizer ;
    ec:constructorArguments ( [ ec:argumentTypeName "se.liu.ida.hefquin.engine.queryplan.utils.LogicalToPhysicalPlanConverter" ;
                ec:constructorArguments ( [ rdf:value false ] [ rdf:value false ] ) ;
                ec:javaClassName "se.liu.ida.hefquin.engine.queryplan.utils.LogicalToPhysicalPlanConverterImpl" ] ) ;
    ec:javaClassName "se.liu.ida.hefquin.engine.queryproc.impl.poptimizer.PhysicalOptimizerWithoutOptimization" .

ec:DefaultPlanCompiler a ec:PlanCompiler ;
    ec:constructorArguments ( [ rdf:value <http://w3id.org/hefquin/engineconf#value:QueryProcContext> ] ) ;
    ec:javaClassName "se.liu.ida.hefquin.engine.queryproc.impl.compiler.PushBasedQueryPlanCompilerImpl" .

ec:DefaultSourcePlanner a ec:SourcePlanner ;
    ec:constructorArguments ( [ rdf:value <http://w3id.org/hefquin/engineconf#value:QueryProcContext> ] ) ;
    ec:javaClassName "se.liu.ida.hefquin.engine.queryproc.impl.srcsel.ServiceClauseBasedSourcePlannerImpl" .

ec:argumentTypeName a rdf:Property ;
    rdfs:label "name of Java class or a Java interface"@en ;
    rdfs:comment "Specifies the full name of a Java class or of a Java interface."@en ;
    rdfs:domain ec:InstantiationBasedConstructorArgument ;
    rdfs:range xsd1:string .

ec:constructorArguments a rdf:Property ;
    rdfs:label "constructor arguments"@en ;
    rdfs:comment "Specifies the list of arguments that must be passed to the constructor of the Java class. Every element of this list is expected to be of type 'ConstructorArgument'."@en ;
    rdfs:domain ec:InstantiableJavaClass ;
    rdfs:range rdf:List .

ec:costModel a rdf:Property ;
    rdfs:label "cost model"@en ;
    rdfs:comment "Specifies the cost model to be used by the query processor. This property is optional because not all configurations of the HeFQUIN query processor use a cost model."@en ;
    rdfs:domain ec:QueryProcessor ;
    rdfs:range ec:CostModel .

ec:elements a rdf:Property ;
    rdfs:label "list elements"@en ;
    rdfs:comment "Specifies the elements to be included in a list that is created as an argument for the constructor of a Java class. Every element of this list is expected to be of type 'InstantiableJavaClass'."@en ;
    rdfs:domain ec:ListBasedConstructorArgument ;
    rdfs:range rdf:List .

ec:elementsTypeName a rdf:Property ;
    rdfs:label "name of Java class or a Java interface"@en ;
    rdfs:comment "Specifies the full name of a Java class or of a Java interface."@en ;
    rdfs:domain ec:ListBasedConstructorArgument ;
    rdfs:range xsd1:string .

ec:executionEngine a rdf:Property ;
    rdfs:label "execution engine"@en ;
    rdfs:comment "Specifies the execution engine to be used by the query processor."@en ;
    rdfs:domain ec:QueryProcessor ;
    rdfs:range ec:ExecutionEngine .

ec:fedAccessMgr a rdf:Property ;
    rdfs:label "federation access manager"@en ;
    rdfs:comment "Specifies the federation access manager to be used in a configuration of the HeFQUIN engine. Every such configuration has only one federation access manager."@en ;
    rdfs:domain ec:HeFQUINEngineConfiguration ;
    rdfs:range ec:FederationAccessManager .

ec:javaClassName a rdf:Property ;
    rdfs:label "name of Java class"@en ;
    rdfs:comment "Specifies the full name of a Java class."@en ;
    rdfs:domain ec:InstantiableJavaClass ;
    rdfs:range xsd1:string .

ec:logicalOptimizer a rdf:Property ;
    rdfs:label "logical optimizer"@en ;
    rdfs:comment "Specifies the logical optimizer to be used by the query planner."@en ;
    rdfs:domain ec:QueryPlanner ;
    rdfs:range ec:LogicalOptimizer .

ec:physicalOptimizer a rdf:Property ;
    rdfs:label "physical optimizer"@en ;
    rdfs:comment "Specifies the physical optimizer to be used by the query planner."@en ;
    rdfs:domain ec:QueryPlanner ;
    rdfs:range ec:PhysicalOptimizer .

ec:planCompiler a rdf:Property ;
    rdfs:label "plan compiler"@en ;
    rdfs:comment "Specifies the plan compiler to be used by the query processor."@en ;
    rdfs:domain ec:QueryProcessor ;
    rdfs:range ec:PlanCompiler .

ec:queryPlanner a rdf:Property ;
    rdfs:label "query planner"@en ;
    rdfs:comment "Specifies the query planner to be used by the query processor."@en ;
    rdfs:domain ec:QueryProcessor ;
    rdfs:range ec:QueryPlanner .

ec:queryProcessor a rdf:Property ;
    rdfs:label "query processor"@en ;
    rdfs:comment "Specifies the query processor to be used in a configuration of the HeFQUIN engine. Every such configuration has only one query processor."@en ;
    rdfs:domain ec:HeFQUINEngineConfiguration ;
    rdfs:range ec:QueryProcessor .

ec:sourcePlanner a rdf:Property ;
    rdfs:label "source planner"@en ;
    rdfs:comment "Specifies the source planner to be used by the query planner."@en ;
    rdfs:domain ec:QueryPlanner ;
    rdfs:range ec:SourcePlanner .

<http://w3id.org/hefquin/engineconf#value:CostModel> a ec:DesignatedArgumentValue .

<http://w3id.org/hefquin/engineconf> rdfs:label "Vocabulary for describing configurations of the HeFQUIN engine"@en ;
    dc:creator "Olaf Hartig" ;
    dc:date "2023-11-29" ;
    dc:format "RDF" ;
    dc:identifier <http://w3id.org/hefquin/engineconf> ;
    dc:title "Vocabulary for describing configurations of the HeFQUIN engine"@en .

<http://w3id.org/hefquin/engineconf#value:ExecServiceForFedAccess> a ec:DesignatedArgumentValue .

<http://w3id.org/hefquin/engineconf#value:QueryProcContext> a ec:DesignatedArgumentValue .

